olty: switch to higher-order semantic types
Also switch experiments, but now we must merge both experiments and introduce
higher-order type members and kinds.

theories/olty.v
@@ -11,26 +11,28 @@ Module Type OLty (Import VS: VlSortsFullSig).
 Include LiftWp VS.
 
 Section olty_limit_preserving.
-  Context `{Σ : gFunctors}.
+  Context `{Σ : gFunctors} {i : nat}.
 
-  Definition envD_persistent (A : envD Σ) := ∀ ρ w, Persistent (A ρ w).
+  Definition hoEnvD_persistent (A : hoEnvD Σ i) := ∀ args ρ w, Persistent (A args ρ w).
 
-  Instance: LimitPreserving envD_persistent.
+  Instance: LimitPreserving hoEnvD_persistent.
   Proof.
+    apply limit_preserving_forall=> args;
     apply limit_preserving_forall=> ρ; apply limit_preserving_forall=> w.
-      apply bi.limit_preserving_Persistent => n ?? H. exact: H.
+    apply bi.limit_preserving_Persistent => n f g Heq. exact: Heq.
   Qed.
 
-  Definition vclosed (A : envD Σ) := ∀ ρ v, A ρ v ⊢ ⌜ nclosed_vl v 0 ⌝.
+  Definition vclosed (A : hoEnvD Σ i) := ∀ args ρ v, A args ρ v ⊢ ⌜ nclosed_vl v 0 ⌝.
 
   Instance: LimitPreserving vclosed.
   Proof.
+    apply limit_preserving_forall=> args;
     apply limit_preserving_forall=> ρ; apply limit_preserving_forall=> w.
     apply limit_preserving_entails; last apply _.
-    solve_proper_ho.
+    move => n f g Heq. exact: Heq.
   Qed.
 
-  Definition restrict A := vclosed A ∧ envD_persistent A.
+  Definition restrict A := vclosed A ∧ hoEnvD_persistent A.
   Global Instance: LimitPreserving restrict.
   Proof.
     apply limit_preserving_and; apply _.
@@ -41,84 +43,86 @@ End olty_limit_preserving.
 "Open Logical TYpes": persistent Iris predicates over environments
 and values. Adapted from
 https://gitlab.mpi-sws.org/iris/examples/blob/d4f4153920ea82617c7222aeeb00b6710d51ee03/theories/logrel_heaplang/ltyping.v#L5. *)
-Record olty Σ := Olty {
-  olty_car :> (var → vl) → vl → iProp Σ;
+Record olty Σ i := Olty {
+  olty_car :> vec vl i → (var → vl) → vl → iProp Σ;
   olty_vclosed : vclosed olty_car;
-  olty_persistent ρ v : Persistent (olty_car ρ v);
+  olty_persistent args ρ v : Persistent (olty_car args ρ v);
 }.
-Global Arguments Olty {_} _%I _ {_}.
-Global Arguments olty_car {_} _ _ _: simpl never.
-Global Arguments olty_vclosed {_} _ _ _ /.
+Global Arguments Olty {_ _} _%I _ {_}.
+Global Arguments olty_car {_ _} _ _ _ _: simpl never.
+Global Arguments olty_vclosed {_ _} _ _ _.
 Bind Scope olty_scope with olty.
 Delimit Scope olty_scope with T.
 Global Existing Instance olty_persistent.
 
 (* Different from normal TyInterp. Better? *)
-Class OTyInterp ty Σ :=
-  oty_interp: ty → olty Σ.
+Class OTyInterp (ty : nat → Type) Σ :=
+  oty_interp : ∀ {i}, ty i → olty Σ i.
+(* Forces inserting coercions to -d>. *)
+Notation oApp := (olty_car : olty _ _ → hoEnvD _ _).
 
-Local Definition testCoerce `(τ : olty Σ) ρ := τ ρ.
+Local Definition testCoerce `(τ : olty Σ 0) := vclose (oApp τ).
 
 Section olty_ofe.
-  Context `{Σ : gFunctors}.
-  Implicit Types (φ : envD Σ) (τ : olty Σ).
+  Context `{Σ : gFunctors} {i : nat}.
+  Implicit Types (φ : hoEnvD Σ i) (τ : olty Σ i).
 
-  Instance olty_equiv : Equiv (olty Σ) := λ A B, A ≡@{envD Σ} B.
-  Instance olty_dist : Dist (olty Σ) := λ n A B, A ≡{n}@{envD Σ}≡ B.
-  Lemma olty_ofe_mixin : OfeMixin (olty Σ).
-  Proof. by apply (iso_ofe_mixin (olty_car : _ → (var → vl) -d> vl -d> _)). Qed.
-  Canonical Structure oltyO := OfeT (olty Σ) olty_ofe_mixin.
+  Instance olty_equiv : Equiv (olty Σ i) := λ A B, oApp A ≡ B.
+  Instance olty_dist : Dist (olty Σ i) := λ n A B, oApp A ≡{n}≡ B.
+  Lemma olty_ofe_mixin : OfeMixin (olty Σ i).
+  Proof. by apply (iso_ofe_mixin oApp). Qed.
+  Canonical Structure oltyO := OfeT (olty Σ i) olty_ofe_mixin.
 
   (* Only needed to define Olty using Iris fixpoints (e.g. for normal recursive types). *)
   Global Instance olty_cofe : Cofe oltyO.
   Proof.
-    set curry_olty : ∀ A, restrict A → olty Σ := λ A '(conj P1 P2), @Olty Σ A P1 P2.
+    set curry_olty : ∀ A, restrict A → olty Σ i := λ A '(conj P1 P2), @Olty Σ i A P1 P2.
     apply (iso_cofe_subtype' restrict curry_olty olty_car) => //.
     - by move => [].
     - by move => ? [].
     - apply _.
   Qed.
 
-  Global Program Instance olty_inhabited : Inhabited (olty Σ) := populate (Olty (λ _ _, False)%I _).
+  Global Program Instance olty_inhabited : Inhabited (olty Σ i) := populate (Olty (λ _ _ _, False)%I _).
   Next Obligation. by unseal=>?. Qed.
 
-  Global Instance olty_car_ne : NonExpansive (@olty_car Σ : olty Σ -> envD Σ).
+  Global Instance olty_car_ne : NonExpansive oApp.
   Proof. intros n f g Heq. apply Heq. Qed.
-  Global Instance lty_car_proper : Proper ((≡) ==> (≡)) (@olty_car Σ : olty Σ -> envD Σ).
+  Global Instance lty_car_proper : Proper ((≡) ==> (≡)) oApp.
   Proof. apply ne_proper, olty_car_ne. Qed.
 
-  Program Definition pack φ (Hvc : vclosed φ) := Olty (λ ρ v, □ φ ρ v)%I _.
+  Program Definition pack φ (Hvc : vclosed φ) := Olty (λ args ρ v, □ φ args ρ v)%I _.
   Next Obligation. rewrite /vclosed; intros. iIntros "?". by iApply Hvc. Qed.
 
   Lemma persistently_id (P : iProp Σ) `{!Persistent P}: □P ⊣⊢ P.
   (* Proof. by iSplit; iIntros. Qed. *)
   Proof. apply: intuitionistic_intuitionistically. Qed.
 
-  Lemma olty_car_pack_id φ (H : vclosed φ) `{∀ ρ v, Persistent (φ ρ v)} :
-    olty_car (pack φ H) ≡@{envD Σ} φ.
+  Lemma olty_car_pack_id φ (H : vclosed φ) `{∀ args ρ v, Persistent (φ args ρ v)} :
+    oApp (pack φ H) ≡ φ.
   Proof.
-    move => ?? /=.
+    move => ??? /=.
     apply: intuitionistic_intuitionistically.
   Qed.
 
   Lemma pack_olty_car_id τ : pack (olty_car τ) (olty_vclosed τ) ≡ τ.
   Proof.
-    move: τ => []?????/=.
+    move: τ => [τ Hp Hvc] args ρ v; rewrite /olty_car/=.
     apply: intuitionistic_intuitionistically.
   Qed.
 
-  Global Instance ids_envD : Ids (envD Σ) := λ _, inhabitant.
-  Global Instance rename_envD : Rename (envD Σ) :=
-    λ r φ ρ, φ (r >>> ρ).
-  Global Instance hsubst_envD : HSubst vl (envD Σ) :=
-    λ sb φ ρ, φ (sb >> ρ).
+  Global Instance ids_hoEnvD : Ids (hoEnvD Σ i) := λ _, inhabitant.
+  Global Instance rename_hoEnvD : Rename (hoEnvD Σ i) :=
+    λ r φ args ρ, φ args (r >>> ρ).
+  Global Instance hsubst_hoEnvD : HSubst vl (hoEnvD Σ i) :=
+    λ sb φ args ρ, φ args (sb >> ρ).
 
-  Ltac renLemmas_envD :=
-    hnf; rewrite /hsubst /hsubst_envD => /= *;
-    try (apply FunctionalExtensionality.functional_extensionality_dep => ?); by asimpl.
+  Ltac renLemmas_hoEnvD :=
+    hnf; rewrite /hsubst /hsubst_hoEnvD => /= *;
+    do 2 (apply FunctionalExtensionality.functional_extensionality_dep => ?); by asimpl.
 
-  Global Instance HSubstLemmas_envD : HSubstLemmas vl (envD Σ).
-  Proof. split => //; renLemmas_envD. Qed.
+  Global Instance HSubstLemmas_hoEnvD : HSubstLemmas vl (hoEnvD Σ i).
+  Proof. split => //; renLemmas_hoEnvD. Qed.
 
   (*
     Since substitution lemmas don't use setoids,
@@ -127,30 +131,30 @@ Section olty_ofe.
 
   Lemma olty_eq τ1 τ2: olty_car τ1 = olty_car τ2 → τ1 = τ2.
   Proof.
-    move: τ1 τ2 => [φ1 ??] [φ2 ??]; rewrite /olty_car.
-    destruct 1. f_equal; exact: ProofIrrelevance.proof_irrelevance.
+    move: τ1 τ2 => [φ1 Hp1 Hvc1] [φ2 Hp2 Hvc2]. rewrite /olty_car /=.
+    intros ->. f_equal; exact: ProofIrrelevance.proof_irrelevance.
   Qed.
 
-  Global Instance ids_olty : Ids (olty Σ) := λ _, inhabitant.
-  Global Program Instance rename_olty : Rename (olty Σ) :=
+  Global Instance ids_olty : Ids (olty Σ i) := λ _, inhabitant.
+  Global Program Instance rename_olty : Rename (olty Σ i) :=
     λ r τ, Olty (rename r (olty_car τ)) _.
   Next Obligation. rewrite /vclosed; intros. exact: olty_vclosed. Qed.
-  Global Program Instance hsubst_olty : HSubst vl (olty Σ) :=
+  Global Program Instance hsubst_olty : HSubst vl (olty Σ i) :=
     λ sb τ, Olty ((olty_car τ).|[sb]) (_ (olty_car τ).|[sb]).
   Next Obligation. rewrite /vclosed; intros. exact: olty_vclosed. Qed.
 
-  Global Instance hsubstLemmas_olty : HSubstLemmas vl (olty Σ).
+  Global Instance hsubstLemmas_olty : HSubstLemmas vl (olty Σ i).
   Proof.
     split=> [s|??|?? s]; apply olty_eq => //; case: s => [φ??];
     rewrite /hsubst /hsubst_olty /olty_car.
     all: trivial using hsubst_id, id_hsubst, hsubst_comp.
   Qed.
 
-(* Global Instance rename_olty2 : Rename (olty Σ) :=
+(* Global Instance rename_olty2 : Rename (olty Σ i) :=
     λ r τ, Olty (λ ρ, τ (r >>> ρ)) (λ ρ, olty_vclosed τ _).
-  Global Instance hsubst_olty2 : HSubst vl (olty Σ) :=
+  Global Instance hsubst_olty2 : HSubst vl (olty Σ i) :=
     λ sb τ, Olty (λ ρ, τ (sb >> ρ)) (λ ρ, olty_vclosed τ _).
-  Global Instance HSubstLemmas_olty2 : HSubstLemmas vl (olty Σ).
+  Global Instance HSubstLemmas_olty2 : HSubstLemmas vl (olty Σ i).
   Proof.
     split=> [s|??|?? s]; apply olty_eq => //; case: s => [φ??];
     (apply functional_extensionality_dep => ?);
@@ -158,47 +162,53 @@ Section olty_ofe.
     all: by asimpl.
   Qed. *)
 
-  Lemma envD_weaken ρ1 ρ2 ρ3 φ :
-    φ.|[upn (length ρ1) (ren (+ length ρ2))] (to_subst (ρ1 ++ ρ2 ++ ρ3))
-    = φ (to_subst (ρ1 ++ ρ3)).
-  Proof. rewrite /hsubst_envD /hsubst to_subst_weaken //. Qed.
+  Lemma hoEnvD_weaken ρ1 ρ2 ρ3 φ args :
+    φ.|[upn (length ρ1) (ren (+ length ρ2))] args (to_subst (ρ1 ++ ρ2 ++ ρ3))
+    = φ args (to_subst (ρ1 ++ ρ3)).
+  Proof. rewrite /hsubst_hoEnvD /hsubst to_subst_weaken //. Qed.
 
-  Lemma envD_subst_up ρ1 ρ2 v φ :
-    φ.|[upn (length ρ1) (v.[ren (+length ρ2)] .: ids)] (to_subst (ρ1 ++ ρ2))
-    ≡ φ (to_subst (ρ1 ++ v :: ρ2)).
-  Proof. rewrite /hsubst_envD /hsubst to_subst_up //. Qed.
+  Lemma hoEnvD_subst_up ρ1 ρ2 v φ args :
+    φ.|[upn (length ρ1) (v.[ren (+length ρ2)] .: ids)] args (to_subst (ρ1 ++ ρ2))
+    ≡ φ args (to_subst (ρ1 ++ v :: ρ2)).
+  Proof. rewrite /hsubst_hoEnvD /hsubst to_subst_up //. Qed.
 
-  Lemma olty_weaken ρ1 ρ2 ρ3 τ :
-    τ.|[upn (length ρ1) (ren (+ length ρ2))] (to_subst (ρ1 ++ ρ2 ++ ρ3))
-    = τ (to_subst (ρ1 ++ ρ3)).
+  Lemma olty_weaken ρ1 ρ2 ρ3 τ args :
+    τ.|[upn (length ρ1) (ren (+ length ρ2))] args (to_subst (ρ1 ++ ρ2 ++ ρ3))
+    = τ args (to_subst (ρ1 ++ ρ3)).
   Proof.
-    (* rewrite /hsubst_olty /hsubst_envD /hsubst /= to_subst_weaken //. *)
+    (* rewrite /hsubst_olty /hsubst_hoEnvD /hsubst /= to_subst_weaken //. *)
     rewrite [@hsubst _ _ hsubst_olty]/hsubst /hsubst_olty /=.
-    exact: envD_weaken.
+    exact: hoEnvD_weaken.
   Qed.
 
-  Lemma envD_weaken_one v φ ρ:
-    φ.|[ren (+1)] (v .: to_subst ρ) = φ (to_subst ρ).
-  Proof. by rewrite (envD_weaken [] [v]). Qed.
+  Lemma hoEnvD_weaken_one v φ ρ args :
+    φ.|[ren (+1)] args (v .: to_subst ρ) = φ args (to_subst ρ).
+  Proof. by rewrite (hoEnvD_weaken [] [v]). Qed.
 
-  Lemma olty_weaken_one v τ ρ:
-    τ.|[ren (+1)] (v .: to_subst ρ) ≡@{vl -d> _} τ (to_subst ρ).
+  Lemma olty_weaken_one v τ ρ args :
+    oApp τ.|[ren (+1)] args (v .: to_subst ρ) ≡ τ args (to_subst ρ).
   Proof. by rewrite (olty_weaken [] [v]). Qed.
 
-  Lemma olty_subst_up ρ1 ρ2 v τ :
-    τ.|[upn (length ρ1) (v.[ren (+length ρ2)] .: ids)] (to_subst (ρ1 ++ ρ2))
-    ≡@{vl -d> _} τ (to_subst (ρ1 ++ v :: ρ2)).
+  Lemma olty_subst_up ρ1 ρ2 v τ args :
+    oApp τ.|[upn (length ρ1) (v.[ren (+length ρ2)] .: ids)] args (to_subst (ρ1 ++ ρ2))
+    ≡ τ args (to_subst (ρ1 ++ v :: ρ2)).
   Proof.
-    (* rewrite /hsubst_olty /hsubst_envD /hsubst /= to_subst_up //. *)
+    (* rewrite /hsubst_olty /hsubst_hoEnvD /hsubst /= to_subst_up //. *)
     rewrite [@hsubst _ _ hsubst_olty]/hsubst /hsubst_olty /=.
-    exact: envD_subst_up.
+    exact: hoEnvD_subst_up.
   Qed.
+End olty_ofe.
 
-  Definition sCtx := list (olty Σ).
+Notation oClose φ := (olty_car φ vnil : envD _).
+Section olty_ofe_2.
+  Context `{Σ : gFunctors} {i : nat}.
+  Implicit Types (φ : hoEnvD Σ i) (τ : olty Σ i).
+
+  Definition sCtx := list (olty Σ 0).
 
   Fixpoint env_oltyped (Γ : sCtx) (ρ : var → vl) : iProp Σ :=
     match Γ with
-    | φ :: Γ' => env_oltyped Γ' ((+1) >>> ρ) ∗ φ ρ (ρ 0)
+    | φ :: Γ' => env_oltyped Γ' ((+1) >>> ρ) ∗ oClose φ ρ (ρ 0)
     | nil => True
     end%I.
 
@@ -209,7 +219,7 @@ Section olty_ofe.
     env_oltyped Γ ρ -∗ ⌜ nclosed_sub (length Γ) 0 ρ ⌝.
   Proof.
     elim: Γ ρ => [|φ Γ IHΓ] ρ /=; [| rewrite IHΓ olty_vclosed ]; iIntros "!% //".
-    - move => [Hclρ Hclp0] [|i /lt_S_n] Hle. exact Hclp0. apply Hclρ, Hle.
+    - move => [Hclρ Hclp0] [|n /lt_S_n] Hle. exact Hclp0. apply Hclρ, Hle.
   Qed.
 
   Lemma env_oltyped_cl_app `{Sort X} (x : X) Γ ρ:
@@ -224,7 +234,7 @@ Section olty_ofe.
 
   Fixpoint env_oltyped_fin (Γ : sCtx) vs : iProp Σ :=
     match Γ, vs with
-    | φ :: Γ', v :: vs => env_oltyped_fin Γ' vs ∗ φ (v .: to_subst vs) v
+    | φ :: Γ', v :: vs => env_oltyped_fin Γ' vs ∗ oClose φ (v .: to_subst vs) v
     | nil, nil => True
     | _, _ => False
     end%I.
@@ -276,9 +286,9 @@ Section olty_ofe.
     by iIntros "!%".
   Qed.
 
-  Lemma interp_env_lookup Γ ρ τ x:
+  Lemma interp_env_lookup Γ ρ (τ : olty Σ 0) x:
     Γ !! x = Some τ →
-    ⟦ Γ ⟧* ρ -∗ τ.|[ren (+x)] (to_subst ρ) (to_subst ρ x).
+    ⟦ Γ ⟧* ρ -∗ oClose τ.|[ren (+x)] (to_subst ρ) (to_subst ρ x).
   Proof.
     elim: Γ ρ x => [//|τ' Γ' IHΓ] [|v ρ] x Hx /=. by iIntros "[]".
     iDestruct 1 as "[Hg Hv]". move: x Hx => [ [->] | x Hx] /=.
@@ -288,38 +298,43 @@ Section olty_ofe.
       iApply (IHΓ ρ x Hx with "Hg").
   Qed.
 
-  Program Definition closed_olty (φ : envD Σ) `{∀ ρ v, Persistent (φ ρ v)} : olty Σ :=
-    Olty (λ ρ v, ⌜ nclosed_vl v 0 ⌝ ∗ φ ρ v)%I _.
-  Next Obligation. iIntros (????) "[$_]". Qed.
+  Program Definition ho_closed_olty {i} (φ : hoEnvD Σ i) `{∀ args ρ v, Persistent (φ args ρ v)} : olty Σ i :=
+    Olty (λ args ρ v, ⌜ nclosed_vl v 0 ⌝ ∗ φ args ρ v)%I _.
+  Next Obligation. iIntros (??????) "[$_]". Qed.
+
+  Definition closed_olty (φ : envD Σ)`{∀ ρ v, Persistent (φ ρ v)} : olty Σ 0 :=
+    ho_closed_olty (vopen φ).
 
   (** We can define once and for all basic "logical" types: top, bottom, and, or, later and μ. *)
-  Definition oTop := closed_olty (λ ρ v, True)%I.
+  Definition oTop : olty Σ i := ho_closed_olty (λ args ρ v, True)%I.
 
-  Program Definition oBot : olty Σ := Olty (λ ρ v, False)%I _.
+  Program Definition oBot : olty Σ i := Olty (λ args ρ v, False)%I _.
   Next Obligation. intros **?**. exact: False_elim. Qed.
 
-  Program Definition oAnd τ1 τ2 : olty Σ := Olty (λ ρ v, τ1 ρ v ∧ τ2 ρ v)%I _.
+  Program Definition oAnd τ1 τ2 : olty Σ i := Olty (λ args ρ v, τ1 args ρ v ∧ τ2 args ρ v)%I _.
   Next Obligation. intros **?**. rewrite olty_vclosed. iIntros "[$ _]". Qed.
 
-  Program Definition oOr τ1 τ2 : olty Σ := Olty (λ ρ v, τ1 ρ v ∨ τ2 ρ v)%I _.
+  Program Definition oOr τ1 τ2 : olty Σ i := Olty (λ args ρ v, τ1 args ρ v ∨ τ2 args ρ v)%I _.
   Next Obligation. intros **?**. rewrite !olty_vclosed. iIntros "[$ | $]". Qed.
 
-  Definition eLater i (φ : envD Σ) : envD Σ := (λ ρ v, ▷^i φ ρ v)%I.
-  Definition oLater τ := closed_olty (eLater 1 τ).
+  Definition eLater n (φ : hoEnvD Σ i) : hoEnvD Σ i := (λ args ρ v, ▷^n φ args ρ v)%I.
+  Definition oLater τ := ho_closed_olty (eLater 1 τ).
 
-  Program Definition oMu τ : olty Σ := Olty (λ ρ v, τ (v .: ρ) v) _.
+  Program Definition ho_oMu {i} (τ : olty Σ i) : olty Σ i := Olty (λ args ρ v, τ args (v .: ρ) v) _.
   Next Obligation. rewrite /vclosed; intros. exact: olty_vclosed. Qed.
 
-  Lemma interp_TMu_ren T ρ v: oMu T.|[ren (+1)] (to_subst ρ) v ≡ T (to_subst ρ) v.
-  Proof. rewrite [_ (oMu _)]/olty_car /= (olty_weaken_one v T ρ v). by []. Qed.
+  Definition oMu (τ : olty Σ 0) : olty Σ 0 := ho_oMu τ.
 
-  Definition interp_expr `{dlangG Σ} (φ : envD Σ) : envPred tm Σ :=
-    λ ρ t, WP t {{ φ ρ }} %I.
+  Lemma interp_TMu_ren (T : olty Σ i) args ρ v: ho_oMu T.|[ren (+1)] args (to_subst ρ) v ≡ T args (to_subst ρ) v.
+  Proof. rewrite [_ (ho_oMu _)]/olty_car /= (olty_weaken_one v T ρ args v). by []. Qed.
+
+  Definition interp_expr `{dlangG Σ} (φ : hoEnvD Σ 0) : envPred tm Σ :=
+    λ ρ t, WP t {{ vclose φ ρ }} %I.
   Global Arguments interp_expr /.
 
   Definition oTSel0 `{dlangG Σ} s σ :=
     closed_olty (λ ρ v, ∃ ψ, s ↗[ σ ] ψ ∧ ▷ □ ψ v)%I.
-End olty_ofe.
+End olty_ofe_2.
 
 Notation "⟦ Γ ⟧*" := (env_oltyped_fin Γ).
 Arguments oltyO : clear implicits.
@@ -329,11 +344,11 @@ Module Type OLtyJudgements (Import VS: VlSortsFullSig).
 Include OLty VS.
 Section judgments.
   Context `{dlangG Σ}.
-  Implicit Types (τ : olty Σ).
+  Implicit Types (τ : olty Σ 0).
 
   Definition step_indexed_ivstp Γ τ1 τ2 i j: iProp Σ :=
     (□∀ ρ v, ⌜ nclosed_vl v 0 ⌝ →
-      ⟦Γ⟧*ρ → (▷^i τ1 (to_subst ρ) v) → ▷^j τ2 (to_subst ρ) v)%I.
+      ⟦Γ⟧*ρ → (▷^i oClose τ1 (to_subst ρ) v) → ▷^j oClose τ2 (to_subst ρ) v)%I.
   Global Arguments step_indexed_ivstp /.
 
   Definition ietp Γ τ e : iProp Σ := (⌜ nclosed e (length Γ) ⌝ ∗
@@ -342,7 +357,7 @@ Section judgments.
 
   Definition step_indexed_ietp Γ τ e i: iProp Σ :=
     (⌜ nclosed e (length Γ) ⌝ ∗ □∀ ρ, ⟦Γ⟧* ρ →
-      interp_expr (λ ρ v, ▷^i τ ρ v) (to_subst ρ) (e.|[to_subst ρ]))%I.
+      interp_expr (eLater i τ) (to_subst ρ) (e.|[to_subst ρ]))%I.
   Global Arguments step_indexed_ietp /.
 
 End judgments.
@@ -353,11 +368,11 @@ Notation "Γ ⊨ [ τ1 , i ]  <: [ τ2 , j ]" := (step_indexed_ivstp Γ τ1 τ2 
 
 Section typing.
   Context `{dlangG Σ}.
-  Implicit Types (τ : olty Σ).
+  Implicit Types (τ : olty Σ 0).
 
-  Lemma iterate_TLater_later i (τ : olty Σ) ρ v:
+  Lemma iterate_TLater_later i τ ρ v:
     nclosed_vl v 0 →
-    (iterate oLater i τ) ρ v ≡ (▷^i τ ρ v)%I.
+    oClose (iterate oLater i τ) ρ v ≡ (vclose (eLater i τ) ρ v).
   Proof.
     elim: i => [|i IHi] // => Hcl. rewrite iterate_S [_ ρ]/olty_car/= /eLater IHi //.
     iSplit; by [iIntros "#[_ $]" | iIntros "$"].
